AwsCryptographyPrimitives/runtimes/java/src/main/java/ECDH/KeyGeneration.java
@@ -1,0 +1,18 @@
+package ECDH;
+
+import Wrappers_Compile.Result;
+import software.amazon.cryptography.primitives.ToDafny;
+import software.amazon.cryptography.primitives.internaldafny.types.ECDHCurveSpec;
+import software.amazon.cryptography.primitives.internaldafny.types.Error;
+import software.amazon.cryptography.primitives.model.OpaqueError;
+
+public class KeyGeneration extends _ExternBase___default {
+
+  public static Result<EccKeyPair, Error> GenerateKeyPair(
+    ECDHCurveSpec ecdhCurveSpec
+  ) {
+    return CreateExternEccKeyGenFailure(
+      ToDafny.Error(OpaqueError.builder().message("Implement me!").build())
+    );
+  }
+}
