AwsCryptographyPrimitives/runtimes/java/src/main/smithy-generated/software/amazon/cryptography/primitives/ToDafny.java
@@ -19,18 +19,25 @@ import software.amazon.cryptography.primitives.internaldafny.types.AES__CTR;
 import software.amazon.cryptography.primitives.internaldafny.types.AES__GCM;
 import software.amazon.cryptography.primitives.internaldafny.types.AesKdfCtrInput;
 import software.amazon.cryptography.primitives.internaldafny.types.CryptoConfig;
+import software.amazon.cryptography.primitives.internaldafny.types.DeriveSharedSecretInput;
+import software.amazon.cryptography.primitives.internaldafny.types.DeriveSharedSecretOutput;
 import software.amazon.cryptography.primitives.internaldafny.types.DigestAlgorithm;
 import software.amazon.cryptography.primitives.internaldafny.types.DigestInput;
+import software.amazon.cryptography.primitives.internaldafny.types.ECDHCurveSpec;
 import software.amazon.cryptography.primitives.internaldafny.types.ECDSASignInput;
 import software.amazon.cryptography.primitives.internaldafny.types.ECDSASignatureAlgorithm;
 import software.amazon.cryptography.primitives.internaldafny.types.ECDSAVerifyInput;
 import software.amazon.cryptography.primitives.internaldafny.types.Error;
 import software.amazon.cryptography.primitives.internaldafny.types.Error_AwsCryptographicPrimitivesError;
+import software.amazon.cryptography.primitives.internaldafny.types.GenerateECCKeyPairInput;
+import software.amazon.cryptography.primitives.internaldafny.types.GenerateECCKeyPairOutput;
 import software.amazon.cryptography.primitives.internaldafny.types.GenerateECDSASignatureKeyInput;
 import software.amazon.cryptography.primitives.internaldafny.types.GenerateECDSASignatureKeyOutput;
 import software.amazon.cryptography.primitives.internaldafny.types.GenerateRSAKeyPairInput;
 import software.amazon.cryptography.primitives.internaldafny.types.GenerateRSAKeyPairOutput;
 import software.amazon.cryptography.primitives.internaldafny.types.GenerateRandomBytesInput;
+import software.amazon.cryptography.primitives.internaldafny.types.GetPublicKeyFromPrivateKeyInput;
+import software.amazon.cryptography.primitives.internaldafny.types.GetPublicKeyFromPrivateKeyOutput;
 import software.amazon.cryptography.primitives.internaldafny.types.GetRSAKeyModulusLengthInput;
 import software.amazon.cryptography.primitives.internaldafny.types.GetRSAKeyModulusLengthOutput;
 import software.amazon.cryptography.primitives.internaldafny.types.HMacInput;
@@ -44,6 +51,8 @@ import software.amazon.cryptography.primitives.internaldafny.types.RSAEncryptInp
 import software.amazon.cryptography.primitives.internaldafny.types.RSAPaddingMode;
 import software.amazon.cryptography.primitives.internaldafny.types.RSAPrivateKey;
 import software.amazon.cryptography.primitives.internaldafny.types.RSAPublicKey;
+import software.amazon.cryptography.primitives.internaldafny.types.ValidatePublicKeyInput;
+import software.amazon.cryptography.primitives.internaldafny.types.ValidatePublicKeyOutput;
 import software.amazon.cryptography.primitives.model.AES_CTR;
 import software.amazon.cryptography.primitives.model.AES_GCM;
 import software.amazon.cryptography.primitives.model.AwsCryptographicPrimitivesError;
@@ -228,6 +237,33 @@ public class ToDafny {
     return new CryptoConfig();
   }
 
+  public static DeriveSharedSecretInput DeriveSharedSecretInput(
+    software.amazon.cryptography.primitives.model.DeriveSharedSecretInput nativeValue
+  ) {
+    DafnySequence<? extends Byte> privateKey;
+    privateKey =
+      software.amazon.smithy.dafny.conversion.ToDafny.Simple.ByteSequence(
+        nativeValue.privateKey()
+      );
+    DafnySequence<? extends Byte> publicKey;
+    publicKey =
+      software.amazon.smithy.dafny.conversion.ToDafny.Simple.ByteSequence(
+        nativeValue.publicKey()
+      );
+    return new DeriveSharedSecretInput(privateKey, publicKey);
+  }
+
+  public static DeriveSharedSecretOutput DeriveSharedSecretOutput(
+    software.amazon.cryptography.primitives.model.DeriveSharedSecretOutput nativeValue
+  ) {
+    DafnySequence<? extends Byte> sharedSecret;
+    sharedSecret =
+      software.amazon.smithy.dafny.conversion.ToDafny.Simple.ByteSequence(
+        nativeValue.sharedSecret()
+      );
+    return new DeriveSharedSecretOutput(sharedSecret);
+  }
+
   public static DigestInput DigestInput(
     software.amazon.cryptography.primitives.model.DigestInput nativeValue
   ) {
@@ -317,6 +353,32 @@ public class ToDafny {
     return success;
   }
 
+  public static GenerateECCKeyPairInput GenerateECCKeyPairInput(
+    software.amazon.cryptography.primitives.model.GenerateECCKeyPairInput nativeValue
+  ) {
+    ECDHCurveSpec eccCurve;
+    eccCurve = ToDafny.ECDHCurveSpec(nativeValue.eccCurve());
+    return new GenerateECCKeyPairInput(eccCurve);
+  }
+
+  public static GenerateECCKeyPairOutput GenerateECCKeyPairOutput(
+    software.amazon.cryptography.primitives.model.GenerateECCKeyPairOutput nativeValue
+  ) {
+    ECDHCurveSpec eccCurve;
+    eccCurve = ToDafny.ECDHCurveSpec(nativeValue.eccCurve());
+    DafnySequence<? extends Byte> privateKey;
+    privateKey =
+      software.amazon.smithy.dafny.conversion.ToDafny.Simple.ByteSequence(
+        nativeValue.privateKey()
+      );
+    DafnySequence<? extends Byte> publicKey;
+    publicKey =
+      software.amazon.smithy.dafny.conversion.ToDafny.Simple.ByteSequence(
+        nativeValue.publicKey()
+      );
+    return new GenerateECCKeyPairOutput(eccCurve, privateKey, publicKey);
+  }
+
   public static GenerateECDSASignatureKeyInput GenerateECDSASignatureKeyInput(
     software.amazon.cryptography.primitives.model.GenerateECDSASignatureKeyInput nativeValue
   ) {
@@ -384,6 +446,33 @@ public class ToDafny {
     RSAPrivateKey privateKey;
     privateKey = ToDafny.RSAPrivateKey(nativeValue.privateKey());
     return new GenerateRSAKeyPairOutput(publicKey, privateKey);
+  }
+
+  public static GetPublicKeyFromPrivateKeyInput GetPublicKeyFromPrivateKeyInput(
+    software.amazon.cryptography.primitives.model.GetPublicKeyFromPrivateKeyInput nativeValue
+  ) {
+    DafnySequence<? extends Byte> privateKey;
+    privateKey =
+      software.amazon.smithy.dafny.conversion.ToDafny.Simple.ByteSequence(
+        nativeValue.privateKey()
+      );
+    return new GetPublicKeyFromPrivateKeyInput(privateKey);
+  }
+
+  public static GetPublicKeyFromPrivateKeyOutput GetPublicKeyFromPrivateKeyOutput(
+    software.amazon.cryptography.primitives.model.GetPublicKeyFromPrivateKeyOutput nativeValue
+  ) {
+    DafnySequence<? extends Byte> privateKey;
+    privateKey =
+      software.amazon.smithy.dafny.conversion.ToDafny.Simple.ByteSequence(
+        nativeValue.privateKey()
+      );
+    DafnySequence<? extends Byte> publicKey;
+    publicKey =
+      software.amazon.smithy.dafny.conversion.ToDafny.Simple.ByteSequence(
+        nativeValue.publicKey()
+      );
+    return new GetPublicKeyFromPrivateKeyOutput(privateKey, publicKey);
   }
 
   public static GetRSAKeyModulusLengthInput GetRSAKeyModulusLengthInput(
@@ -672,6 +761,30 @@ public class ToDafny {
     return new RSAPublicKey(lengthBits, pem);
   }
 
+  public static ValidatePublicKeyInput ValidatePublicKeyInput(
+    software.amazon.cryptography.primitives.model.ValidatePublicKeyInput nativeValue
+  ) {
+    DafnySequence<? extends Byte> privateKey;
+    privateKey =
+      software.amazon.smithy.dafny.conversion.ToDafny.Simple.ByteSequence(
+        nativeValue.privateKey()
+      );
+    DafnySequence<? extends Byte> publicKey;
+    publicKey =
+      software.amazon.smithy.dafny.conversion.ToDafny.Simple.ByteSequence(
+        nativeValue.publicKey()
+      );
+    return new ValidatePublicKeyInput(privateKey, publicKey);
+  }
+
+  public static ValidatePublicKeyOutput ValidatePublicKeyOutput(
+    software.amazon.cryptography.primitives.model.ValidatePublicKeyOutput nativeValue
+  ) {
+    Boolean success;
+    success = (nativeValue.success());
+    return new ValidatePublicKeyOutput(success);
+  }
+
   public static Error Error(AwsCryptographicPrimitivesError nativeValue) {
     DafnySequence<? extends Character> message;
     message =
@@ -703,6 +816,37 @@ public class ToDafny {
             "Cannot convert " +
             nativeValue +
             " to software.amazon.cryptography.primitives.internaldafny.types.DigestAlgorithm."
+          );
+        }
+    }
+  }
+
+  public static ECDHCurveSpec ECDHCurveSpec(
+    software.amazon.cryptography.primitives.model.ECDHCurveSpec nativeValue
+  ) {
+    switch (nativeValue) {
+      case ECC_NIST_P256:
+        {
+          return ECDHCurveSpec.create_ECC__NIST__P256();
+        }
+      case ECC_NIST_P384:
+        {
+          return ECDHCurveSpec.create_ECC__NIST__P384();
+        }
+      case ECC_NIST_P521:
+        {
+          return ECDHCurveSpec.create_ECC__NIST__P521();
+        }
+      case SM2:
+        {
+          return ECDHCurveSpec.create_SM2();
+        }
+      default:
+        {
+          throw new RuntimeException(
+            "Cannot convert " +
+            nativeValue +
+            " to software.amazon.cryptography.primitives.internaldafny.types.ECDHCurveSpec."
           );
         }
     }
