AwsCryptographyPrimitives/runtimes/java/src/main/smithy-generated/software/amazon/cryptography/primitives/model/GenerateECCKeyPairOutput.java
@@ -1,0 +1,121 @@
+// Copyright Amazon.com Inc. or its affiliates. All Rights Reserved.
+// SPDX-License-Identifier: Apache-2.0
+// Do not modify this file. This file is machine generated, and any changes to it will be overwritten.
+package software.amazon.cryptography.primitives.model;
+
+import java.nio.ByteBuffer;
+import java.util.Objects;
+
+public class GenerateECCKeyPairOutput {
+
+  private final ECDHCurveSpec eccCurve;
+
+  private final ByteBuffer privateKey;
+
+  private final ByteBuffer publicKey;
+
+  protected GenerateECCKeyPairOutput(BuilderImpl builder) {
+    this.eccCurve = builder.eccCurve();
+    this.privateKey = builder.privateKey();
+    this.publicKey = builder.publicKey();
+  }
+
+  public ECDHCurveSpec eccCurve() {
+    return this.eccCurve;
+  }
+
+  public ByteBuffer privateKey() {
+    return this.privateKey;
+  }
+
+  public ByteBuffer publicKey() {
+    return this.publicKey;
+  }
+
+  public Builder toBuilder() {
+    return new BuilderImpl(this);
+  }
+
+  public static Builder builder() {
+    return new BuilderImpl();
+  }
+
+  public interface Builder {
+    Builder eccCurve(ECDHCurveSpec eccCurve);
+
+    ECDHCurveSpec eccCurve();
+
+    Builder privateKey(ByteBuffer privateKey);
+
+    ByteBuffer privateKey();
+
+    Builder publicKey(ByteBuffer publicKey);
+
+    ByteBuffer publicKey();
+
+    GenerateECCKeyPairOutput build();
+  }
+
+  static class BuilderImpl implements Builder {
+
+    protected ECDHCurveSpec eccCurve;
+
+    protected ByteBuffer privateKey;
+
+    protected ByteBuffer publicKey;
+
+    protected BuilderImpl() {}
+
+    protected BuilderImpl(GenerateECCKeyPairOutput model) {
+      this.eccCurve = model.eccCurve();
+      this.privateKey = model.privateKey();
+      this.publicKey = model.publicKey();
+    }
+
+    public Builder eccCurve(ECDHCurveSpec eccCurve) {
+      this.eccCurve = eccCurve;
+      return this;
+    }
+
+    public ECDHCurveSpec eccCurve() {
+      return this.eccCurve;
+    }
+
+    public Builder privateKey(ByteBuffer privateKey) {
+      this.privateKey = privateKey;
+      return this;
+    }
+
+    public ByteBuffer privateKey() {
+      return this.privateKey;
+    }
+
+    public Builder publicKey(ByteBuffer publicKey) {
+      this.publicKey = publicKey;
+      return this;
+    }
+
+    public ByteBuffer publicKey() {
+      return this.publicKey;
+    }
+
+    public GenerateECCKeyPairOutput build() {
+      if (Objects.isNull(this.eccCurve())) {
+        throw new IllegalArgumentException(
+          "Missing value for required field `eccCurve`"
+        );
+      }
+      if (Objects.isNull(this.privateKey())) {
+        throw new IllegalArgumentException(
+          "Missing value for required field `privateKey`"
+        );
+      }
+      if (Objects.isNull(this.publicKey())) {
+        throw new IllegalArgumentException(
+          "Missing value for required field `publicKey`"
+        );
+      }
+      return new GenerateECCKeyPairOutput(this);
+    }
+  }
+}
