AwsCryptographyPrimitives/runtimes/java/src/main/smithy-generated/software/amazon/cryptography/primitives/model/GetPublicKeyFromPrivateKeyInput.java
@@ -1,0 +1,65 @@
+// Copyright Amazon.com Inc. or its affiliates. All Rights Reserved.
+// SPDX-License-Identifier: Apache-2.0
+// Do not modify this file. This file is machine generated, and any changes to it will be overwritten.
+package software.amazon.cryptography.primitives.model;
+
+import java.nio.ByteBuffer;
+import java.util.Objects;
+
+public class GetPublicKeyFromPrivateKeyInput {
+
+  private final ByteBuffer privateKey;
+
+  protected GetPublicKeyFromPrivateKeyInput(BuilderImpl builder) {
+    this.privateKey = builder.privateKey();
+  }
+
+  public ByteBuffer privateKey() {
+    return this.privateKey;
+  }
+
+  public Builder toBuilder() {
+    return new BuilderImpl(this);
+  }
+
+  public static Builder builder() {
+    return new BuilderImpl();
+  }
+
+  public interface Builder {
+    Builder privateKey(ByteBuffer privateKey);
+
+    ByteBuffer privateKey();
+
+    GetPublicKeyFromPrivateKeyInput build();
+  }
+
+  static class BuilderImpl implements Builder {
+
+    protected ByteBuffer privateKey;
+
+    protected BuilderImpl() {}
+
+    protected BuilderImpl(GetPublicKeyFromPrivateKeyInput model) {
+      this.privateKey = model.privateKey();
+    }
+
+    public Builder privateKey(ByteBuffer privateKey) {
+      this.privateKey = privateKey;
+      return this;
+    }
+
+    public ByteBuffer privateKey() {
+      return this.privateKey;
+    }
+
+    public GetPublicKeyFromPrivateKeyInput build() {
+      if (Objects.isNull(this.privateKey())) {
+        throw new IllegalArgumentException(
+          "Missing value for required field `privateKey`"
+        );
+      }
+      return new GetPublicKeyFromPrivateKeyInput(this);
+    }
+  }
+}
