AwsCryptographyPrimitives/runtimes/net/Extern/ECDH.cs
@@ -1,0 +1,25 @@
+// Copyright Amazon.com Inc. or its affiliates. All Rights Reserved.
+// SPDX-License-Identifier: Apache-2.0
+
+
+using software.amazon.cryptography.primitives.internaldafny.types;
+using Wrappers_Compile;
+using icharseq = Dafny.ISequence<char>;
+using ibyteseq = Dafny.ISequence<byte>;
+using byteseq = Dafny.Sequence<byte>;
+using _IError = software.amazon.cryptography.primitives.internaldafny.types._IError;
+using Error_Opaque = software.amazon.cryptography.primitives.internaldafny.types.Error_Opaque;
+
+namespace ECDH
+{
+    public partial class KeyGeneration
+    {
+        public static _IResult<EccKeyPair, _IError> GenerateKeyPair(_IECDHCurveSpec x)
+        {
+            return Result<EccKeyPair, _IError>
+                .create_Failure(new Error_Opaque("Implement me!"));
+
+        }
+
+    }
+}
