AwsCryptographyPrimitives/runtimes/net/Generated/ValidatePublicKeyInput.cs
@@ -1,0 +1,37 @@
+// Copyright Amazon.com Inc. or its affiliates. All Rights Reserved.
+// SPDX-License-Identifier: Apache-2.0
+// Do not modify this file. This file is machine generated, and any changes to it will be overwritten.
+using System;
+using AWS.Cryptography.Primitives;
+namespace AWS.Cryptography.Primitives
+{
+    public class ValidatePublicKeyInput
+    {
+        private System.IO.MemoryStream _privateKey;
+        private System.IO.MemoryStream _publicKey;
+        public System.IO.MemoryStream PrivateKey
+        {
+            get { return this._privateKey; }
+            set { this._privateKey = value; }
+        }
+        public bool IsSetPrivateKey()
+        {
+            return this._privateKey != null;
+        }
+        public System.IO.MemoryStream PublicKey
+        {
+            get { return this._publicKey; }
+            set { this._publicKey = value; }
+        }
+        public bool IsSetPublicKey()
+        {
+            return this._publicKey != null;
+        }
+        public void Validate()
+        {
+            if (!IsSetPrivateKey()) throw new System.ArgumentException("Missing value for required property 'PrivateKey'");
+            if (!IsSetPublicKey()) throw new System.ArgumentException("Missing value for required property 'PublicKey'");
+
+        }
+    }
+}
