AwsCryptographyPrimitives/src/ECDH.dfy
@@ -1,0 +1,37 @@
+// Copyright Amazon.com Inc. or its affiliates. All Rights Reserved.
+// SPDX-License-Identifier: Apache-2.0
+
+include "../Model/AwsCryptographyPrimitivesTypes.dfy"
+
+module {:extern "ECDH"} ECDH {
+  import opened Wrappers
+  import opened UInt = StandardLibrary.UInt
+  import Types = AwsCryptographyPrimitivesTypes
+
+  datatype EccKeyPair = EccKeyPair(privateKey: seq<uint8>, publicKey: seq<uint8>)
+
+  method GenerateEccKeyPair(
+    input: Types.GenerateECCKeyPairInput
+  ) returns (output: Result<Types.GenerateECCKeyPairOutput, Types.Error>)
+  {
+    var keyPair :- ExternEccKeyGen(input.eccCurve);
+
+    return Success(Types.GenerateECCKeyPairOutput(
+                     eccCurve := input.eccCurve,
+                     privateKey := keyPair.privateKey,
+                     publicKey := keyPair.publicKey
+                   ));
+  }
+
+  method {:extern "ECDH.KeyGeneration", "GenerateKeyPair"} ExternEccKeyGen(
+    s: Types.ECDHCurveSpec
+  ) returns (res: Result<EccKeyPair, Types.Error>)
+
+  function method CreateExternEccKeyGenSuccess(output: EccKeyPair): Result<EccKeyPair, Types.Error> {
+    Success(output)
+  }
+
+  function method CreateExternEccKeyGenFailure(error: Types.Error): Result<EccKeyPair, Types.Error> {
+    Failure(error)
+  }
+} 
