AwsCryptographyPrimitives/Model/ecdh.smithy
@@ -1,0 +1,96 @@
+namespace aws.cryptography.primitives
+
+@enum([
+  {
+    name: "ECC_NIST_P256",
+    value: "ECC_NIST_P256",
+  },
+  {
+    name: "ECC_NIST_P384",
+    value: "ECC_NIST_P384",
+  },
+  {
+    name: "ECC_NIST_P521",
+    value: "ECC_NIST_P521",
+  },
+  {
+    // TODO: come back and double check this is the spec kms uses
+    name: "SM2",
+    value: "SM2",
+  },
+])
+string ECDHCurveSpec
+
+operation GenerateECCKeyPair {
+    input: GenerateECCKeyPairInput,
+    output: GenerateECCKeyPairOutput,
+    errors: []
+}
+
+operation GetPublicKeyFromPrivateKey {
+    input: GetPublicKeyFromPrivateKeyInput,
+    output: GetPublicKeyFromPrivateKeyOutput,
+    errors: []
+}
+
+operation ValidatePublicKey {
+    input: ValidatePublicKeyInput,
+    output: ValidatePublicKeyOutput,
+    errors: []
+}
+
+operation DeriveSharedSecret {
+    input: DeriveSharedSecretInput,
+    output: DeriveSharedSecretOutput,
+    errors: []
+}
+
+structure GenerateECCKeyPairInput {
+    @required
+    eccCurve: ECDHCurveSpec 
+}
+
+structure GenerateECCKeyPairOutput {
+    @required
+    eccCurve: ECDHCurveSpec,
+    @required
+    privateKey: Blob,
+    @required
+    publicKey: Blob 
+}
+
+structure GetPublicKeyFromPrivateKeyInput {
+    @required
+    privateKey: Blob,
+}
+
+structure GetPublicKeyFromPrivateKeyOutput {
+    @required
+    privateKey: Blob,
+    @required
+    publicKey: Blob 
+}
+
+structure ValidatePublicKeyInput {
+    @required
+    privateKey: Blob,
+    @required
+    publicKey: Blob 
+}
+
+structure ValidatePublicKeyOutput {
+    @required
+    success: Boolean,
+}
+
+structure DeriveSharedSecretInput {
+    @required
+    privateKey: Blob,
+    @required
+    publicKey: Blob 
+}
+
+structure DeriveSharedSecretOutput {
+    @required
+    sharedSecret: Blob
+}
