AwsCryptographyPrimitives/Model/primitives.smithy
@@ -27,6 +27,10 @@ service AwsCryptographicPrimitives {
     GenerateECDSASignatureKey,
     ECDSASign,
     ECDSAVerify,
+    GenerateECCKeyPair,
+    GetPublicKeyFromPrivateKey,
+    ValidatePublicKey,
+    DeriveSharedSecret
   ],
   errors: [AwsCryptographicPrimitivesError]
 }
